\documentclass[a4paper,12pt]{article}
\input{/usr/share/LaTeX-ToolKit/template.tex}
\title{}
\author{沈威宇}
\date{\temtoday}
\pagestyle{empty}
\begin{document}
\temdoc
\section*{Hyperbolic Function Cheat Sheet}
\[\ba
\sinh(x)&=\frac{e^x-e^{-x}}{2}\\
\cosh(x)&=\frac{e^x+e^{-x}}{2}\\
\tanh(x)&=\frac{e^{2x}-1}{e^{2x}+1}\\
\coth(x)&=\frac{e^{2x}+1}{e^{2x}-1}\\
\sech(x)&=\frac{2}{e^x+e^{-x}}\\
\csch(x)&=\frac{2}{e^x-e^{-x}}
\ea\]
\[\ba
\operatorname{arcsinh}(x)&= \ln\left(x+\sqrt{x^2+1}\right)\\
\operatorname{arccosh}(x)&= \ln\left(x+\sqrt{x^2-1}\right),\quad x\geq 1\\
\operatorname{arctanh}(x)&= \frac{1}{2}\ln\left(\frac{1+x}{1-x}\right),\quad\abs{x}<1\\
\operatorname{arccoth}(x)&= \frac{1}{2}\ln\left(\frac{x+1}{x-1}\right),\quad\abs{x}>1\\
\operatorname{arcsech}(x)&= \ln\left(\frac{1}{x}+\frac{\sqrt{1-x^2}}{x}\right),\quad 0<x\leq 1\\
\operatorname{arccsch}(x)&= \ln\left(\frac{1}{x}+\frac{\sqrt{1+x^2}}{\abs{x}}\right),\quad x\neq 0
\ea\]
\[\ba
\sinh\theta\csch\theta=1\\
\cosh\theta\sech\theta=1\\
\tanh\theta\coth\theta=1
\ea\]
\[\ba
\tanh\theta\cosh\theta=\sinh\theta\\
\sinh\theta\coth\theta=\cosh\theta\\
\sinh\theta\sech\theta=\tanh\theta\\
\cosh\theta\csch\theta=\coth\theta\\
\tanh\theta\csch\theta=\sech\theta\\
\coth\theta\sech\theta=\csch\theta
\ea\]
\[\ba
\sinh^2\theta+1=\cosh^2\theta\\
\tanh^2\theta+\sech^2\theta=1\\
\coth^2\theta+\csch^2\theta=1
\ea\]
\[\ba\cosh x+\sinh x=e^x\\
\cosh x-\sinh x=e^{-x}\ea\]
\[\ba
\sinh\theta=\frac{2\tanh\frac{\theta}{2}}{1-\tanh^2\frac{\theta}{2}}\\
\cosh\theta=\frac{1+\tanh^2\frac{\theta}{2}}{1-\tanh^2\frac{\theta}{2}}\\
\tanh\theta=\frac{2\tanh\frac{\theta}{2}}{1+\tanh^2\frac{\theta}{2}}
\ea\]
\[\ba
\sinh 2\theta&=2\sinh\theta\cosh\theta\\
\cosh 2\theta &=1+2\sinh^2\theta\\
&=2\cosh^2\theta-1\\
&=\cosh^2\theta+\sinh^2\theta
\ea\]
\[\ba
\sinh\frac{\theta}{2}  &=\operatorname{sgn}(\theta)\sqrt{\frac{\cosh\theta-1}{2}}\\
\cosh\frac{\theta}{2}  &=\sqrt{\frac{\cosh\theta+1}{2}}\\
\tanh\frac{\theta}{2}  &=\operatorname{sgn}(\theta)\sqrt{\frac{\cosh\theta-1}{\cosh\theta+1}}\\
&=\frac{\sinh\theta}{\cosh\theta+1}\\
&=\frac{\cosh\theta-1}{\sinh\theta}\\
&=\frac{\sinh\theta+\cosh\theta-1}{\sinh\theta+\cosh\theta+1}\\
&=\coth\theta-\csch\theta
\ea\]
\[\sinh 3\theta=3\sinh\theta+4\sinh^3\theta\]
\[\cosh 3\theta=4\cosh^3\theta-3\cosh\theta\]
\[\tanh 3\theta=\frac{3\tanh\theta+\tanh^3\theta}{1+3\tanh^2\theta}\]
\[\sinh\qty(\alpha +\beta)=\sinh\alpha\cosh\beta +\cosh\alpha\sinh\beta\]
\[\sinh\qty(\alpha -\beta)=\sinh\alpha\cosh\beta -\cosh\alpha\sinh\beta\]
\[\cosh\qty(\alpha +\beta)=\cosh\alpha\cosh\beta +\sinh\alpha\sinh\beta\]
\[\cosh\qty(\alpha -\beta)=\cosh\alpha\cosh\beta -\sinh\alpha\sinh\beta\]
\[\tanh\qty(\alpha +\beta)=\frac{\tanh\alpha+\tanh\beta}{1+\tanh\alpha\tanh\beta}\]
\[\tanh\qty(\alpha -\beta)=\frac{\tanh\alpha-\tanh\beta}{1-\tanh\alpha\tanh\beta}\]
\[\coth\qty(\alpha +\beta)=\frac{\coth\alpha\coth\beta +1}{\coth\alpha +\coth\beta}\]
\[\coth\qty(\alpha -\beta)=\frac{\coth\alpha\coth\beta -1}{\coth\beta -\coth\alpha}\]
\[\sech\qty(\alpha +\beta)=\frac{\sech\alpha\sech\beta}{1+\tanh\alpha\tanh\beta}=\frac{\csch\alpha\csch\beta}{\coth\alpha\coth\beta+1}\]
\[\sech\qty(\alpha -\beta)=\frac{\sech\alpha\sech\beta}{1-\tanh\alpha\tanh\beta}=\frac{\csch\alpha\csch\beta}{\coth\alpha\coth\beta-1}\]
\[\csch\qty(\alpha +\beta)=\frac{\csch\alpha\csch\beta}{\coth\alpha+\coth\beta}=\frac{\sech\alpha\sech\beta}{\tanh\alpha+\tanh\beta}\]
\[\csch\qty(\alpha -\beta)=\frac{\csch\alpha\csch\beta}{\coth\beta-\coth\alpha}=\frac{\sech\alpha\sech\beta}{\tanh\alpha-\tanh\beta}\]
\[\sinh^2\theta=\frac{\tanh^2\theta}{1-\tanh^2\theta}\]
\[\cosh^2\theta=\frac{1}{1-\tanh^2\theta}\]
\[\coth^2\theta=\frac{1}{\tanh^2\theta}\]
\[\sech^2\theta=1-\tanh^2\theta\]
\[\csch^2\theta=\frac{1-\tanh^2\theta}{\tanh^2\theta}\]
\bma
\sinh\alpha +\sinh\beta &= 2\sinh\frac{\alpha +\beta}{2}\cosh\frac{\alpha -\beta}{2}\\
\sinh\alpha -\sinh\beta &= 2\cosh\frac{\alpha +\beta}{2}\sinh\frac{\alpha -\beta}{2}\\
\cosh\alpha +\cosh\beta &= 2\cosh\frac{\alpha +\beta}{2}\cosh\frac{\alpha -\beta}{2}\\
\cosh\alpha -\cosh\beta &= 2\sinh\frac{\alpha +\beta}{2}\sinh\frac{\alpha -\beta}{2}
\eam
\bma
2\sinh\alpha\cosh\beta &= \sinh(\alpha +\beta)+\sinh(\alpha -\beta)\\
2\cosh\alpha\sinh\beta &= \sinh(\alpha +\beta)-\sinh(\alpha -\beta)\\
2\cosh\alpha\cosh\beta &= \cosh(\alpha +\beta)+\cosh(\alpha -\beta)\\
2\sinh\alpha\sinh\beta &= \cosh(\alpha +\beta)-\cosh(\alpha -\beta)
\eam
\end{document}